Some work on min+max using the MinMaxSpec first.

ADTExamples/MinPlusMax.v
@@ -325,108 +325,6 @@ Section MinMaxExample.
                                 ))
       | idtac]; cbv beta in *; simpl in * .
 
-  Definition delegateADTSiR' (or : multiset)
-             (nr : multiset * Rep MinMaxSpec) :=
-    or = fst nr /\ fst nr = snd nr.
-
-  Definition delegateADTSiR'' (or : multiset * multiset)
-             (nr : multiset * Rep MinMaxImpl) :=
-    fst or = fst nr /\ SiR (fst nr) (snd nr).
-
-  Definition MinPlusMaxImpl' (defaultValue : nat)
-  : Sharpened MinPlusMaxSpec.
-  Proof.
-    (** Add a MinMax instance to the representation so we can delegate to it. *)
-    unfold MinPlusMaxSpec, NatTwoBinOpSpec, two_op_spec.
-    (** Split out the [Pick]s in the MinPlusMax Observer. *)
-    hone' observer "MinPlusMax"%string using _.
-    { intros; subst.
-      set_evars; simpl in *.
-      setoid_rewrite refineEquiv_split_func_ex2'.
-      (* The following three tactics are seriously inscrutable. *)
-      subst_body.
-      rewrite_hyp.
-      higher_order_2_reflexivity. }
-    hone representation' using delegateADTSiR'.
-    (** Rewrite the "Min" and then "Max" [Pick] in the MinPlusMax Observer. *)
-    unfold delegateADTSiR'.
-    hone' observer "MinPlusMax"%string using _.
-    { intros; subst.
-      set_evars; simpl in *.
-      unfold refine; intros.
-      econstructor; intros; intuition; subst.
-      replace ({a : nat | bin_op_spec ge _ (fst r_n) n a})
-      with (callObs MinMaxSpec "Max" (snd r_n) n) by (rewrite H3; reflexivity).
-      replace ({a : nat | bin_op_spec le _ (fst r_n) n a})
-      with (callObs MinMaxSpec "Min" (snd r_n) n) by (rewrite H3; reflexivity).
-      subst_body.
-      eapply H0.
-    }
-    (* Rewrite insert to use MinMaxSpec's insert. *)
-    hone' mutator "Insert"%string using
-    (fun (r : multiset * multiset) x =>
-       (r1 <- callMut MinPlusMaxSpec "Insert" (fst r) x;
-        r2 <- callMut MinMaxSpec "Insert" (snd r) x;
-        ret (r1, r2))).
-    { intros; subst.
-      unfold refine; intros; inversion_by computes_to_inv; subst;
-      econstructor.
-      unfold add_spec in *.
-      econstructor; intros; intuition; subst.
-      econstructor; split.
-      econstructor; split.
-      instantiate (1 := (x, x0)); split; simpl; eauto.
-      apply functional_extensionality; simpl; eauto.
-      apply functional_extensionality; simpl; eauto.
-      intros; rewrite H1, H0, H3; auto.
-      econstructor; eauto.
-    }
-    hone representation' using delegateADTSiR''.
-    hone' observer "MinPlusMax"%string using (fun r_n n =>
-          (a <- {n' : nat | bin_op_spec le defaultSpec (snd r_n) n n'};
-           a' <- {n' : nat | bin_op_spec ge defaultSpec (snd r_n) n n'};
-           ret (a + a')))%obsDef.
-    { unfold delegateADTSiR''; intros; subst.
-      set_evars; simpl in *.
-      unfold refine; intros.
-      econstructor; intros; intuition; subst.
-      subst_body.
-      rewrite_hyp.
-      eapply H0.
-      intros.
-      simpl
-      econstructor; split; eauto.
-      simpl.
-      split
-
-      unfold add_spec oi
-      autorefine.
-
-    econstructor; intros; try reflexivity.
-
-      subst.
-      unfold delegateADTSiR; simpl.
-      setoid_rewrite remove_forall_eq0.
-      setoid_rewrite remove_exists_and_eq0.
-      setoid_rewrite refineEquiv_pick_eq'.
-      autorewrite with refine_monad.
-      eapply refine_pick.
-      intros.
-      constructor.
-      inversion_by computes_to_inv.
-      subst; simpl.
-      destruct_head sig.
-      inversion_by computes_to_inv.
-      trivial. }
-    - finish sharpening.
-  Defined.
-
-  (* Show the term derived above as a sanity check. *)
-  Goal (forall b, ObserverMethods (projT1 (MinPlusMaxImpl 0))
-                                 {| bstring := "MinPlusMax" |} = b).
-    simpl.
-  Abort.
-
   Definition MinPlusMaxImpl (defaultValue : nat)
   : Sharpened MinPlusMaxSpec.
   Proof.
@@ -450,16 +348,13 @@ Section MinMaxExample.
     (** Rewrite the "Min" and then "Max" [Pick] in the MinPlusMax Observer. *)
     dubiously specialized hone ∑-observer "MinPlusMax"%string  rewriting with observer "Min"%string.
     dubiously specialized hone ∑-observer "MinPlusMax"%string  rewriting with observer "Max"%string.
-
-
-
     hone'' ∑-mutator "Insert"%string using
            (fun (r : {nr : multiset * Rep MinMaxImpl | MinMaxSiR (fst nr) (snd nr)}) x =>
               (r1 <- { v : { v | callMut MinPlusMaxSpec "Insert" (fst (proj1_sig r)) x ↝ v } | True };
                r2 <- { v : { v | callMut MinMaxImpl "Insert" (snd (proj1_sig r)) x ↝ v } | True};
                ret (exist (fun nr => MinMaxSiR (fst nr) (snd nr)) (`r1, `r2) (helper_SiR_preserved _ r1 r2) ))).
-
-      subst.
+    admit.
+(*      subst.
       unfold delegateADTSiR; simpl.
       setoid_rewrite remove_forall_eq0.
       setoid_rewrite remove_exists_and_eq0.
@@ -472,9 +367,232 @@ Section MinMaxExample.
       subst; simpl.
       destruct_head sig.
       inversion_by computes_to_inv.
-      trivial. }
+      trivial. } *)
     - finish sharpening.
   Defined.
+
+  (* An attempt to delegate to the reference spec,
+     then refine the delegate ADT to the implementation. *)
+
+  Definition delegateSpecSiR (or : multiset)
+             (nr : multiset * Rep MinMaxSpec) :=
+    or = fst nr /\ or = snd nr.
+
+  Arguments delegateSpecSiR _ _ / .
+
+  Definition delegateImplSiR (or : multiset * multiset)
+             (nr : multiset * Rep MinMaxImpl) :=
+    fst or = fst nr /\ SiR (snd or) (snd nr).
+
+  Arguments delegateImplSiR _ _ / .
+
+  Lemma refineMinMaxObs {Rep' : Type -> Type}
+        {Dom Cod : Type}
+        (proj : forall A, Rep' A -> A)
+        (SiR' : Rep' (Rep MinMaxSpec) -> Rep' (Rep MinMaxImpl) -> Prop)
+        (bod : forall (adt : ADT MinMaxSig),
+                 observerMethodType (Rep adt) Dom Cod)
+  : (forall or nr, SiR' or nr -> SiR (proj _ or) (proj _ nr))
+    -> (refineObserver SiR (bod MinMaxSpec)
+                       (bod MinMaxImpl))
+    -> refineObserver eq (absObserverMethod SiR' (fun r => (bod MinMaxSpec (proj _ r))))
+                   (fun r => bod MinMaxImpl (proj _ r)).
+  Proof.
+    simpl; intros; subst; econstructor; intros; eauto.
+    eapply H0; eauto.
+  Qed.
+
+  Lemma refineMinMaxMut {Rep' : Type -> Type}
+        {Dom : Type}
+        (proj : forall A, Rep' A -> A)
+        (SiR' : Rep' (Rep MinMaxSpec) -> Rep' (Rep MinMaxImpl) -> Prop)
+        (bod : forall (adt : ADT MinMaxSig),
+                 mutatorMethodType (Rep' (Rep adt)) Dom)
+  : (refineMutator SiR' (bod MinMaxSpec)
+                      (bod MinMaxImpl))
+    -> refineMutator eq (absMutatorMethod SiR' (bod MinMaxSpec))
+                  (bod MinMaxImpl).
+  Proof.
+    simpl; intros; subst; econstructor; intros; eauto.
+    econstructor; intros.
+    generalize (H _ _ _ H1 _ H0); intros; inversion_by computes_to_inv.
+    eauto.
+  Qed.
+
+  Lemma refine_elim_forall
+        {A B : Type}
+        (P : A -> Prop)
+        (P' : A -> B -> Prop)
+        (b : Comp B)
+  : (forall a,
+       P a
+       -> refine {b | P' a b} b)
+    -> refine {b | forall a, P a -> P' a b} b.
+  Proof.
+    intros; econstructor; intros.
+    generalize (H _ H1 _ H0); intros; inversion_by computes_to_inv;
+    eauto.
+  Qed.
+
+  Lemma duplicate_bind {A : Type}
+        (a : Comp A)
+  : (forall x x', computes_to a x -> computes_to a x' -> x = x')
+    -> refineEquiv (a' <- a; ret (a', a'))
+                (a' <- a; a'' <- a; ret (a', a'')).
+  Proof.
+    split; unfold refine; intros; inversion_by computes_to_inv;
+    subst; repeat econstructor; subst; eauto.
+    erewrite (H _ _ H1 H2); econstructor.
+  Qed.
+
+  Tactic Notation "swap" "representation" constr(adt) "with" constr(adt') "under" constr(SiR') :=
+    let A := match goal with  |- Sharpened ?A => constr:(A) end in
+    lazymatch A with
+      | @BuildADT ?Rep' ?mutSigs ?obsSigs ?mutDefs ?obsDefs
+        => let ASig := constr:(BuildADTSig mutSigs obsSigs) in
+           let MutatorIndex' := (eval simpl in (MutatorIndex ASig)) in
+           let ObserverIndex' := (eval simpl in (ObserverIndex ASig)) in
+           let ObserverDomCod' := (eval simpl in (ObserverDomCod ASig)) in
+           eapply SharpenStep
+    end;
+  cbv beta in *; simpl in * .
+
+
+    Lemma swap_rep 
+    : 
+      forall 
+        Sig Sig'
+        (ClientADT : ADT Sig -> ADT Sig')
+        (adt adt' : ADT Sig)
+        (SiR' : Rep (ClientADT adt) -> Rep (ClientADT adt') -> Prop),
+      (forall mutIdx : MutatorIndex Sig',
+         refineMutator SiR' 
+                       (MutatorMethods (ClientADT adt) mutIdx) 
+                       (MutatorMethods (ClientADT adt') mutIdx))
+      -> (forall obsIdx : ObserverIndex Sig',
+            refineObserver SiR' 
+                           (ObserverMethods (ClientADT adt) obsIdx) 
+                           (ObserverMethods (ClientADT adt') obsIdx))
+      -> refineADT (ClientADT adt) (ClientADT adt').
+    Proof.
+      intros.
+      destruct (ClientADT adt); destruct (ClientADT adt').
+      eapply refineADT_Build_ADT_Rep with (SiR := SiR'); eauto.
+    Qed.
+
+  Definition MinPlusMaxImpl' (defaultValue : nat)
+  : Sharpened MinPlusMaxSpec.
+  Proof.
+    clear refineMutatorPreservesSiR.
+    (** Split out the [Pick]s in the MinPlusMax Observer. *)
+    unfold MinPlusMaxSpec, NatTwoBinOpSpec, two_op_spec.
+    hone' observer "MinPlusMax"%string using _; simpl.
+    { intros; subst.
+      set_evars. simpl in *.
+      setoid_rewrite refineEquiv_split_func_ex2'.
+      (* This sequence of tactics is inscrutable. *)
+      subst_body.
+      rewrite_hyp.
+      higher_order_2_reflexivity.
+    }
+    (** Add a MinMax instance to the representation so we can delegate to it. *)
+    hone representation' using delegateSpecSiR.
+    (** Rewrite the "Min" and then "Max" [Pick] in the MinPlusMax Observer. *)
+    hone' observer "MinPlusMax"%string using _.
+    { intros; subst.
+      set_evars. simpl in *.
+      (* Split the /\ *)
+      apply refine_elim_forall; intros; intuition; subst.
+      rewrite H2.
+      (* Rewrite with a call to Min *)
+      replace ({a : nat | bin_op_spec le _ (snd r_n) n a})
+      with ((callObs MinMaxSpec "Min") (snd r_n) n) by reflexivity.
+      (* Rewrite with a call to Max *)
+      replace ({a : nat | bin_op_spec ge _ (snd r_n) n a})
+      with ((callObs MinMaxSpec "Max") (snd r_n) n) by reflexivity.
+      (* Again, inscrutable. *)
+      subst_body.
+      rewrite_hyp.
+      higher_order_2_reflexivity.
+    }
+    (* Rewrite insert to use MinMaxSpec's insert. *)
+    hone' mutator "Insert"%string using _.
+    { intros; subst.
+      set_evars. simpl in *.
+      setoid_rewrite refineEquiv_pick_eq'; autorewrite with refine_monad.
+      apply refine_elim_forall; intros; intuition; subst.
+      (* Pull of the first 'Insert' Picks. *)
+      rewrite refineEquiv_split_ex.
+      rewrite refineEquiv_pick_computes_to_and.
+      autorewrite with refine_monad.
+      (* Delegate insert to MinMax ADT*)
+      rewrite H2.
+      replace {m' : multiset | add_spec (snd r_n) n m'}
+      with (callMut MinMaxSpec "Insert" (snd r_n) n) by reflexivity.
+      (* Clean up second Pick. *)
+      setoid_rewrite <- refineEquiv_split_ex.
+      setoid_rewrite remove_exists_eql_and.
+      setoid_rewrite refineEquiv_pick_pair.
+      setoid_rewrite refineEquiv_pick_eq'.
+      repeat setoid_rewrite refineEquiv_bind_unit.
+      rewrite duplicate_bind;
+        [ | simpl; intros; inversion_by computes_to_inv;
+          apply functional_extensionality; intros; rewrite H0, H1;
+          reflexivity].
+      rewrite <- H2 at 1.
+      subst_body.
+      higher_order_2_reflexivity.
+    }
+    (* Swap representations. *)
+    eapply SharpenStep.
+    (* Do the swap. We should have a 'swap representation' 
+       tactic  to do the pattern matching. *)
+    eapply (@swap_rep MinMaxSig _
+                          (fun adt => 
+                             (ADTRep (multiset * Rep adt)
+      { def mut "Insert" (p : rep, n: nat) : rep := 
+          a' <- (callMut MinPlusMaxSpec "Insert") (fst p) n;
+          a'' <- (callMut adt "Insert") (snd p) n;
+          ret (a', a'') ;
+        def obs "MinPlusMax" (p : rep, n : nat) : nat := 
+          {b : nat |
+          (a <- (callObs adt "Min") (snd p) n ;
+           a' <- (callObs adt "Max") (snd p) n;
+           ret (a + a')) ↝ b}  })%ADT) MinMaxSpec MinMaxImpl
+           delegateImplSiR).
+    (* Show the mutator swap is valid. This is fairly boilerplate. *)
+    {
+      intros; simpl; unfold ith_obligation_1, ith_obligation_2; simpl.
+      destruct mutIdx as  [ ? [ [? | [ ] ] ] ]; subst; simpl.
+      intros; intuition; subst.
+      setoid_rewrite <- (refineMutator_MinMaxSiR {| bstring := "Insert"%string |} _ _ n H1).
+      rewrite H0; autorewrite with refine_monad.
+      repeat (f_equiv; unfold pointwise_relation; intros;
+              autorewrite with refine_monad; simpl). 
+      unfold refine; intros; inversion_by computes_to_inv;
+      subst; econstructor; simpl; auto.
+    }
+    (* Show the observer swap is valid. This is fairly boilerplate. *)
+    {
+      intros; simpl; unfold ith_obligation_1, ith_obligation_2; simpl.
+      destruct obsIdx as  [ ? [ [? | [ ] ] ] ]; subst; simpl. 
+      intros; intuition; subst.
+      repeat rewrite refineEquiv_pick_computes_to.
+      rewrite (refineObserver_MinMaxSiR {| bstring := "Min"%string |} _ _ n H1).
+      f_equiv; unfold pointwise_relation; intros.
+      autorewrite with refine_monad; simpl;
+      rewrite (refineObserver_MinMaxSiR {| bstring := "Max"%string |} _ _ n H1); f_equiv.
+    }
+    - finish sharpening.
+  Defined.
+
+  (* Show the term derived above as a sanity check. *)
+  Goal (forall b, ObserverMethods (projT1 (MinPlusMaxImpl' 0))
+                                 {| bstring := "MinPlusMax" |} = b).
+  intros; simpl.
+  unfold ObserverMethods; cbv beta.
+  Abort.
+
 
   (* Show the term derived above as a sanity check. *)
   Goal (forall b, ObserverMethods (projT1 (MinPlusMaxImpl 0))
